src/Interpreter.fst
@@ -530,258 +530,8 @@ let rec compileCirc (gexp, cs) =
     | Err s -> Err s
     | Val c' -> compileCirc c'
 
-(* Garbage-collected reversible circuit compilation -- experimental *)
-(*
-type qubit =
-  { id   : int;
-    ival : BoolExp;
-    cval : BoolExp }
-
-val null_q : qubit
-val get_subst : Total.t int qubit -> int -> Tot int
-val data_q : int -> Tot qubit
-val anc_q  : int -> Tot qubit
-
-let nullq = { id = 0; ival = BFalse; cval = BFalse }
-let get_subst m = fun i -> (m i).id
-let data_q i = { id = i; ival = BVar i; cval = BFalse }
-let anc_q i  = { id = i; ival = BFalse; cval = BFalse }
-
-type circGCState =
-  { top    : int;
-    ah     : AncHeap;
-    gates  : list Gate;
-    symtab : Total.t int qubit }
-
-val circGC       : circGCState -> int -> Tot circGCState
-val circGCInit   : circGCState
-val circGCAlloc  : circGCState -> BoolExp -> Tot (int * circGCState)
-val circGCAssign : circGCState -> int -> BoolExp -> Tot circGCState
-val circGCEval   : circGCState -> state -> int -> Tot bool
-
-// The garbage collector needs to:
-//  -compile the current value in place (i.e. ival + cval + cval = ival),
-//  -if the qubit is an ancilla, push it back onto the heap, and
-//  -update the current value of all other bits by substituting q.id with ival + cval
-val garbageCollect : circGCState -> qubit -> Tot circGCState
-let garbageCollect cs q = 
-  let (ah', res, ancs, circ) = compileBexp cs.ah q.id q.cval in
-  let ah'' = if q.ival = BFalse then insert ah' q.id else ah' in
-  let f q' = 
-    let subq = fun v -> if v = q.id then BXor (q.ival, q.cval) else BVar v in
-      { id = q'.id; ival = q'.ival; cval = simplify (substBexp q'.cval subq) }
-  in
-  let symtab' = mapVal f cs.symtab in
-    { top = cs.top; ah = ah''; gates = cs.gates @ circ; symtab = symtab' }
-
-let circGCInit = { top = 0; ah = emptyHeap; gates = []; subs = constMap nullq;
-symtab = constMap nullq }
-let circGCAlloc cs bexp = 
-  let bexp' = simplify (substVar bexp (get_subst cs.symtab)) in
-  let (ah', bit) = popMin cs.ah in
-  let (ah'', res, ancs, circ') = compileBexp ah' bit bexp' in
-  let q = { id = bit; ival = BFalse; cval = bexp' } in
-  let top' = cs.top + 1 in
-  let gates' = cs.gates @ circ' in
-  let symtab' = update cs.symtab cs.top q in
-  (cs.top, {top = top'; ah = ah''; gates = gates'; symtab = symtab'})
-let circGCAssign cs l bexp =
-  let q = lookup cs.symtab l in
-  let bexp' = simplify (substVar bexp (get_subst cs.symtab)) in
-  let bexpfac = factorAs bexp' q.id in
-  match (q.cval, bexpfac) with
-    | (BFalse, _)      -> // substitute q.id with BFalse, compile in place
-      let bexp'' = substBexp bexp' (fun v -> if v = q.id then BFalse else BVar v) in
-      let (ah', res, ancs, circ) = compileBexp cs.ah q.id bexp'' in
-      let q' = { id = q.id; ival = q.ival; cval = bexp'' } in
-        {top = cs.top; ah = ah'; gates = cs.gates @ circ; symtab = update cs.symtab l q' }
-    | (_, Some bexp'') -> // compile in place, substitute q.id with q.id \oplus bexp''
-      let (ah', res, ancs, circ') = compileBexp cs.ah q.id bexp'' in
-      let q' = { id = q.id; ival = q.ival; cval = simplify (BXor (q.cval, bexp'')) } in
-      let f b = 
-        let subq = fun v -> if v = q.id then BXor (BVar q.id, bexp'') else BVar v in
-          { id = b.id; ival = b.ival; cval = simplify (substBexp b.cval subq) }
-      in
-      let symtab' = update (mapVal f cs.symtab) l q' in
-        {top = cs.top; ah = ah'; gates = cs.gates @ circ'; symtab = update cs.symtab l q' }
-    | _                -> // Compile out of place, clean q.id
-      let (ah', res, ancs, circ') = compileBexp_oop cs.ah bexp' in
-      let q' = { id = res; ival = BFalse; cval = bexp' } in
-      let cs' = { top = cs.top; ah = ah'; gates = cs.gates @ circ'; symtab = update cs.symtab l q' } in
-        garbageCollect cs' q
-let circGCEval cs st i = false
-
-let circGCInterp = {
-  alloc = circGCAlloc;
-  assign = circGCAssign;
-  eval = circGCEval
-}
-
-val allocNcircGC : list GExpr * circGCState -> i:int ->
-  Tot (list GExpr * circGCState) (decreases i)
-let rec allocNcircGC (locs, cs) i =
-  if i <= 0 then (List.rev locs, cs)
-  else
-    let (ah', res) = popMin cs.ah in
-    let cs' = { top = cs.top + 1;
-                ah = ah';
-                gates = cs.gates;
-                symtab = update cs.symtab cs.top (data_q res) }
-    in
-      allocNcircGC (((LOC cs.top)::locs), cs') (i-1)
-
-val allocTycircGC : GType -> circGCState -> Tot (result (GExpr * circGCState))
-let allocTycircGC ty cs = match ty with
-  | GBool ->
-    let (ah', res) = popMin cs.ah in
-    let cs' = { top = cs.top + 1;
-                ah = ah';
-                gates = cs.gates;
-                symtab = update cs.symtab cs.top (data_q res) }
-    in
-      Val (LOC cs.top, cs')
-  | GArray n ->
-    let (locs, st') = allocNcircGC ([], cs) n in
-      Val (ARRAY locs, st')
-  | _ -> Err "Invalid parameter type for circuit generation"
-
-val lookup_Lst_gc : Total.t int qubit -> lst:(list GExpr){isVal_lst lst} -> Tot (list int)
-let rec lookup_Lst_gc symtab lst = match lst with
-  | [] -> []
-  | (LOC l)::xs -> ((lookup symtab l).id)::(lookup_Lst_gc symtab xs)
-
-val compileGCCirc : config circGCState -> Dv (result (list int * list Gate))
-let rec compileGCCirc (gexp, cs) =
-  if isVal gexp then match gexp with
-    | UNIT -> Val ([], [])
-    | LAMBDA (x, ty, t) ->
-      begin match allocTycircGC ty cs with
-        | Err s -> Err s
-        | Val (v, cs') -> compileGCCirc (substGExpr t x v, cs')
-      end
-    | LOC l ->
-      let res = lookup cs.symtab l in
-        Val ([res.id], cs.gates)
-    | ARRAY lst ->
-      let res = lookup_Lst_gc cs.symtab lst in
-        Val (res, cs.gates)
-  else match (step (gexp, cs) circGCInterp) with
-    | Err s -> Err s
-    | Val c' -> compileGCCirc c'
-
-
-(* Dependence graph interpretation -- unfinished *)
-type depGraphState = (int * int) * (depGraph * (Total.t address rID))
-
-val depGraphInterp : interpretation depGraphState
-let depGraphInterp fs ((atop, rtop), (nodes, dep)) = match fs with
-  | Xor a1 a2 ->
-    bind (lookup dep a1) (fun r1 ->
-    bind (lookup dep a2) (fun r2 ->
-      let nodes'  = (Rinit)::nodes in
-      let nodes'' = (Rbexp (BXor (BVar r1) (BVar r2)) rtop)::nodes' in
-        Val (atop, ((atop+1, rtop+2), (nodes'', update dep atop (rtop+1))))))
-  | And a1 a2 ->
-    bind (lookup dep a1) (fun r1 ->
-    bind (lookup dep a2) (fun r2 ->
-      let nodes'  = (Rinit)::nodes in
-      let nodes'' = (Rbexp (BAnd (BVar r1) (BVar r2)) rtop)::nodes' in
-        Val (atop, ((atop+1, rtop+2), (nodes'', update dep atop (rtop+1))))))
-  | Not a ->
-    bind (lookup dep a) (fun r ->
-      let nodes'  = (Rinit)::nodes in
-      let nodes'' = (Rbexp (BNot (BVar r)) rtop)::nodes' in
-        Val (atop, ((atop+1, rtop+2), (nodes'', update dep atop (rtop+1)))))
-  | Bl b ->
-    let nodes' = (Rinit)::nodes in
-    let (rtop', nodes'') = match b with
-      | false -> (rtop, nodes')
-      | true  -> (rtop+1, (Rbexp (BNot (BVar rtop)) rtop)::nodes')
-    in
-      Val (atop, ((atop+1, rtop'+1), (nodes'', update dep atop rtop')))
-  | Asn a1 a2 -> bind (lookup dep a2) (fun r ->
-    Val (atop, ((atop, rtop), (nodes, update dep a1 r))))
-  | Cln a -> bind (lookup dep a) (fun r ->
-    Val (atop, ((atop, rtop+1), ((Rterm r)::nodes, update dep a rtop))))
-
-val computeGraph : GExpr -> result (valconfig depGraphState)
-let computeGraph gexp = eval_rec (gexp, [], ((0, 0), ([], []))) depGraphInterp
-*)
 
 (** Verification utilities *)
-(*
-val step_preservation : 
-  #state:Type -> #state':Type -> 
-  gexp:GExpr -> st:state -> st':state' -> init:Total.t int bool ->
-  pred:(state -> state' -> Total.t int bool -> Type) ->
-  h1:(forall st st' init. pred st st' init ==> 
-                        
-  Lemma (requires (state_equiv st st' init))
-        (ensures
-          (is_Err (step (gexp, st) boolInterp) /\ is_Err (step (gexp, st') bexpInterp)) \/
-          (is_Val (step (gexp, st) boolInterp) /\ is_Val (step (gexp, st') bexpInterp) /\
-          (fst (getVal (step (gexp, st) boolInterp)) =
-           fst (getVal (step (gexp, st') bexpInterp)) /\
-          state_equiv (snd (getVal (step (gexp, st) boolInterp)))
-                      (snd (getVal (step (gexp, st') bexpInterp)))
-                      init)))
-  (decreases %[gexp;1])
-val step_preservation_lst : lst:list GExpr -> st:boolState -> st':BExpState -> init:state ->
-  Lemma (requires (state_equiv st st' init))
-        (ensures
-          (is_Err (step_lst (lst, st) boolInterp) /\ is_Err (step_lst (lst, st') bexpInterp)) \/
-          (is_Val (step_lst (lst, st) boolInterp) /\ is_Val (step_lst (lst, st') bexpInterp) /\
-          (fst (getVal (step_lst (lst, st) boolInterp)) =
-           fst (getVal (step_lst (lst, st') bexpInterp)) /\
-          state_equiv (snd (getVal (step_lst (lst, st) boolInterp)))
-                      (snd (getVal (step_lst (lst, st') bexpInterp)))
-                      init)))
-  (decreases %[lst;0])
-let rec state_equiv_step gexp st st' init = match gexp with
-  | LET (x, t1, t2) ->
-    state_equiv_step t1 st st' init
-  | LAMBDA (x, ty, t) -> ()
-  | APPLY (t1, t2) ->
-    state_equiv_step t1 st st' init;
-    state_equiv_step t2 st st' init
-  | SEQUENCE (t1, t2) ->
-    state_equiv_step t1 st st' init
-  | ASSIGN (t1, t2) ->
-    state_equiv_step t1 st st' init;
-    state_equiv_step t2 st st' init;
-    if (isVal t1 && isBexp t2) then
-      begin match t1 with
-        | LOC l -> state_equiv_assign st st' init l (get_bexp t2)
-        | _ -> ()
-      end
-  | XOR (t1, t2) ->
-    state_equiv_step t1 st st' init;
-    state_equiv_step t2 st st' init
-  | AND (t1, t2) ->
-    state_equiv_step t1 st st' init;
-    state_equiv_step t2 st st' init
-  | BOOL b -> ()
-  | APPEND (t1, t2) ->
-    state_equiv_step t1 st st' init;
-    state_equiv_step t2 st st' init
-  | ROT (i, t) ->
-    state_equiv_step t st st' init
-  | SLICE (t, i, j) ->
-    state_equiv_step t st st' init
-  | ARRAY lst ->
-    state_equiv_step_lst lst st st' init
-  | GET_ARRAY (t, i) ->
-    state_equiv_step t st st' init
-  | ASSERT t ->
-    state_equiv_step t st st' init
-  | BEXP bexp -> state_equiv_alloc st st' init bexp
-  | _ -> ()
-and state_equiv_step_lst lst st st' init = match lst with
-  | [] -> ()
-  | x::xs ->
-    state_equiv_step x st st' init;
-    state_equiv_step_lst xs st st' init
-*)
 
 (* Originally this was done polymorphically (using a general notion of
    equivalence of states and a proof that the interpreter preserves equivalence
@@ -884,7 +634,7 @@ and state_equiv_step_lst lst st st' init = match lst with
     state_equiv_step x st st' init;
     state_equiv_step_lst xs st st' init
 
-// Correctness of circuit compilation
+(* Correctness of circuit compilation *)
 type circ_equiv (st:boolState) (cs:circState) (init:state) =
   fst st = cs.top /\
   zeroHeap (evalCirc cs.gates init) cs.ah /\
@@ -999,7 +749,7 @@ let circ_equiv_assign st cs init l bexp =
         eval_commutes_subst_circ_oop st cs bexp bexp' init
       in
       ()
-    | Some bexp'' ->
+    | Some bexp'' -> (* TODO: Fix this, doesn't pass anymore *)
       let (ah', res, ancs, circ') = compileBexp cs.ah l' bexp'' in
       let zeroHeap_lem =
         factorAs_correct bexp' l' init';
@@ -1011,20 +761,19 @@ let circ_equiv_assign st cs init l bexp =
         zeroHeap_subset init' cs.ah cs'.ah;
         zeroHeap_st_impl init' cs'.ah circ'
       in
-      let preservation =
-        //admitP(forall i. not (i = l) ==> boolEval st' init i = circEval cs' init i);
+      let preservation = //admitP(forall i. not (i = l) ==> boolEval st' init i = circEval cs' init i);
         compile_mods cs.ah l' bexp'';
         eval_mod init' circ'
       in
-      let correctness =
+      let correctness = //admitP(b2t(lookup (snd st') l = lookup (evalCirc circ' init') (lookup cs'.subs l)))
         admitP(b2t(boolEval st' init l = circEval cs' init l));
         eval_commutes_subst_circ st cs bexp bexp'' init l l'
-        //admitP(b2t(lookup (snd st') l = lookup (evalCirc circ' init') (lookup cs'.subs l)))
-        //factorAs_correct bexp' l' init'
       in
         //admitP(forall i. boolEval st' init i = circEval cs' init i);
       ()
 
+
+(* TODO: Fix this, doesn't pass anymore *)
 val circ_equiv_step : gexp:GExpr -> st:boolState -> st':circState -> init:state ->
   Lemma (requires (circ_equiv st st' init))
         (ensures
@@ -1057,13 +806,13 @@ let rec circ_equiv_step gexp st st' init = match gexp with
   | SEQUENCE (t1, t2) ->
     circ_equiv_step t1 st st' init;
     circ_equiv_step t2 st st' init
-  | ASSIGN (t1, t2) -> admit () (*
-    if      not (isVal t1)  then admit() //circ_equiv_step t1 st st' init
-    else if not (isBexp t2) then admit() //circ_equiv_step t2 st st' init
-    else
+  | ASSIGN (t1, t2) ->
+    circ_equiv_step t1 st st' init
+    circ_equiv_step t2 st st' init
+    if (isVal t1 && isBexp t2) then
       begin match t1 with
-        | LOC l -> admit()//; circ_equiv_assign st st' init l (get_bexp t2)
-        | _ -> admit ()
+        | LOC l -> circ_equiv_assign st st' init l (get_bexp t2)
+        | _ -> ()
       end
   | XOR (t1, t2) ->
     circ_equiv_step t1 st st' init;
@@ -1085,10 +834,84 @@ let rec circ_equiv_step gexp st st' init = match gexp with
     circ_equiv_step t st st' init
   | ASSERT t ->
     circ_equiv_step t st st' init
-  | BEXP bexp -> circ_equiv_alloc st st' init bexp *)
-  | _ -> admit ()
+  | BEXP bexp -> circ_equiv_alloc st st' init bexp
+  | _ -> ()
 and circ_equiv_step_lst lst st st' init = match lst with
   | [] -> ()
   | x::xs ->
     circ_equiv_step x st st' init;
     circ_equiv_step_lst xs st st' init
+
+(* 
+val step_preservation : 
+  #state:Type -> #state':Type -> 
+  gexp:GExpr -> st:state -> st':state' -> init:Total.t int bool ->
+  pred:(state -> state' -> Total.t int bool -> Type) ->
+  h1:(forall st st' init. pred st st' init ==> 
+                        
+  Lemma (requires (state_equiv st st' init))
+        (ensures
+          (is_Err (step (gexp, st) boolInterp) /\ is_Err (step (gexp, st') bexpInterp)) \/
+          (is_Val (step (gexp, st) boolInterp) /\ is_Val (step (gexp, st') bexpInterp) /\
+          (fst (getVal (step (gexp, st) boolInterp)) =
+           fst (getVal (step (gexp, st') bexpInterp)) /\
+          state_equiv (snd (getVal (step (gexp, st) boolInterp)))
+                      (snd (getVal (step (gexp, st') bexpInterp)))
+                      init)))
+  (decreases %[gexp;1])
+val step_preservation_lst : lst:list GExpr -> st:boolState -> st':BExpState -> init:state ->
+  Lemma (requires (state_equiv st st' init))
+        (ensures
+          (is_Err (step_lst (lst, st) boolInterp) /\ is_Err (step_lst (lst, st') bexpInterp)) \/
+          (is_Val (step_lst (lst, st) boolInterp) /\ is_Val (step_lst (lst, st') bexpInterp) /\
+          (fst (getVal (step_lst (lst, st) boolInterp)) =
+           fst (getVal (step_lst (lst, st') bexpInterp)) /\
+          state_equiv (snd (getVal (step_lst (lst, st) boolInterp)))
+                      (snd (getVal (step_lst (lst, st') bexpInterp)))
+                      init)))
+  (decreases %[lst;0])
+let rec state_equiv_step gexp st st' init = match gexp with
+  | LET (x, t1, t2) ->
+    state_equiv_step t1 st st' init
+  | LAMBDA (x, ty, t) -> ()
+  | APPLY (t1, t2) ->
+    state_equiv_step t1 st st' init;
+    state_equiv_step t2 st st' init
+  | SEQUENCE (t1, t2) ->
+    state_equiv_step t1 st st' init
+  | ASSIGN (t1, t2) ->
+    state_equiv_step t1 st st' init;
+    state_equiv_step t2 st st' init;
+    if (isVal t1 && isBexp t2) then
+      begin match t1 with
+        | LOC l -> state_equiv_assign st st' init l (get_bexp t2)
+        | _ -> ()
+      end
+  | XOR (t1, t2) ->
+    state_equiv_step t1 st st' init;
+    state_equiv_step t2 st st' init
+  | AND (t1, t2) ->
+    state_equiv_step t1 st st' init;
+    state_equiv_step t2 st st' init
+  | BOOL b -> ()
+  | APPEND (t1, t2) ->
+    state_equiv_step t1 st st' init;
+    state_equiv_step t2 st st' init
+  | ROT (i, t) ->
+    state_equiv_step t st st' init
+  | SLICE (t, i, j) ->
+    state_equiv_step t st st' init
+  | ARRAY lst ->
+    state_equiv_step_lst lst st st' init
+  | GET_ARRAY (t, i) ->
+    state_equiv_step t st st' init
+  | ASSERT t ->
+    state_equiv_step t st st' init
+  | BEXP bexp -> state_equiv_alloc st st' init bexp
+  | _ -> ()
+and state_equiv_step_lst lst st st' init = match lst with
+  | [] -> ()
+  | x::xs ->
+    state_equiv_step x st st' init;
+    state_equiv_step_lst xs st st' init
+*)
